To prove Binet's Formula, we will employ methods from linear algebra and calculus, specifically involving characteristic equations and eigenvectors. Binet's Formula provides an explicit expression for the \( n \)-th Fibonacci number, \( F_n \), in terms of the golden ratio \( \phi \) and its conjugate. The formula is given by:

$$
F_n = \frac{\phi^n - (1 - \phi)^n}{\sqrt{5}},
$$
where \( $$ \phi = \frac{1 + \sqrt{5}}{2} $$\) is the golden ratio.

### Step 1: The Fibonacci Sequence as a Linear Recurrence

The Fibonacci sequence is defined by the recurrence relation \( F_n = F_{n-1} + F_{n-2} \) with initial conditions \( F_0 = 0 \) and \( F_1 = 1 \). This can be represented in matrix form as:

$$
\begin{pmatrix}
F_{n} \\
F_{n-1}
\end{pmatrix}
=
\begin{pmatrix}
1 & 1 \\
1 & 0
\end{pmatrix}
\begin{pmatrix}
F_{n-1} \\
F_{n-2}
\end{pmatrix}.
$$

### Step 2: Diagonalization of the Matrix

Let \( $$A = \begin{pmatrix} 1 & 1 \\ 1 & 0 \end{pmatrix}$$ \). We find the eigenvalues of \( A \) by solving the characteristic equation \( $$\det(A - \lambda I) = 0 $$\), where \( I \) is the identity matrix. This yields:

$$
\det\begin{pmatrix}
1 - \lambda & 1 \\
1 & -\lambda
\end{pmatrix}
= 0
\implies
\lambda^2 - \lambda - 1 = 0.
$$

The solutions to this quadratic equation are the golden ratio \( \phi = \frac{1 + \sqrt{5}}{2} \) and its conjugate \( $$\psi = \frac{1 - \sqrt{5}}{2} $$\).

### Step 3: Eigenvectors and Diagonalization

For each eigenvalue \( \lambda_i \) (where \( \lambda_i \) is either \( \phi \) or \( \psi \)), we find an eigenvector \( v_i \) such that \( Av_i = \lambda_i v_i \). This allows us to express \( A \) as \( A = PDP^{-1} \), where \( D \) is a diagonal matrix of eigenvalues and \( P \) is a matrix of corresponding eigenvectors.

### Step 4: Expressing \( F_n \) in Terms of \( \phi \) and \( \psi \)

Using the diagonalization, we can express the \( n \)-th power of \( A \) as:

$$
A^n = PD^nP^{-1}.
$$

Applying this to the vector \( \begin{pmatrix} F_1 \\ F_0 \end{pmatrix} \) and using the initial conditions \( F_0 = 0 \) and \( F_1 = 1 \), we find an explicit form for \( F_n \) in terms of \( \phi \) and \( \psi \).

### Step 5: Simplification to Binet's Formula

After some algebraic manipulation, considering the specific eigenvectors and eigenvalues, we can simplify the expression to Binet's formula:

$$
F_n = \frac{\phi^n - \psi^n}{\sqrt{5}},
$$
where \( \psi \) is the conjugate of \( \phi \), \( $$ \psi = \frac{1 - \sqrt{5}}{2} $$\).

### Conclusion

Thus, Binet's Formula is derived from the linear algebraic representation of the Fibonacci sequence, using the concept of eigenvalues and eigenvectors. This formula provides a direct way to calculate the \( n \)-th Fibonacci number without recourse to the recursive definition of the sequence.


## The Algebra in Between
Of course, let's follow the format rigorously. We'll revisit the algebraic manipulations connecting the diagonalization of the matrix to Binet's Formula, ensuring all mathematical notation is within the $$...$$ format.

### Step 1: Finding Eigenvectors
For each eigenvalue \( \lambda \) (where \( \lambda \) is either \( \phi \) or \( \psi \)), we find an eigenvector \( v \) such that 
$$
Av = \lambda v. 
$$
Solving this will provide us with the eigenvectors.

### Step 2: Constructing the Matrix \( P \)
Let \( v_\phi \) and \( v_\psi \) be the eigenvectors corresponding to \( \phi \) and \( \psi \), respectively. The matrix \( P \) is formed by placing these eigenvectors as its columns:
$$
P = \begin{pmatrix} v_\phi & v_\psi \end{pmatrix}.
$$

### Step 3: Diagonal Matrix \( D \)
The diagonal matrix \( D \) consists of the eigenvalues:
$$
D = \begin{pmatrix} \phi & 0 \\ 0 & \psi \end{pmatrix}.
$$

### Step 4: Matrix Power
Given that 
$$
A^n = PD^nP^{-1}, 
$$
we calculate \( A^n \) by raising \( D \) to the \( n \)-th power and then multiplying by \( P \) and \( P^{-1} \). The \( n \)-th power of \( D \) is straightforward:
$$
D^n = \begin{pmatrix} \phi^n & 0 \\ 0 & \psi^n \end{pmatrix}.
$$

### Step 5: Applying to Initial Conditions
Applying \( A^n \) to the initial condition vector 
$$
\begin{pmatrix} 1 \\ 0 \end{pmatrix},
$$ 
we get
$$
\begin{pmatrix} F_{n} \\ F_{n-1} \end{pmatrix} = PD^nP^{-1} \begin{pmatrix} 1 \\ 0 \end{pmatrix}.
$$

### Step 6: Algebraic Manipulation
Expanding this expression and simplifying, using the specific forms of \( P \) and \( P^{-1} \) (based on the eigenvectors of \( A \)), we obtain an explicit expression for \( F_n \). After simplification, this results in:
$$
F_n = \frac{\phi^n - \psi^n}{\phi - \psi}.
$$
Since \( \phi - \psi = \sqrt{5} \), the formula simplifies to Binet's Formula:
$$
F_n = \frac{\phi^n - \psi^n}{\sqrt{5}}.
$$

### Conclusion
This detailed algebraic manipulation demonstrates the transition from the matrix representation of the Fibonacci sequence to Binet's Formula, offering a direct and non-recursive method for calculating Fibonacci numbers. The crucial aspect lies in utilizing the eigenvalues and eigenvectors of the matrix representing the Fibonacci recurrence relationship.